src/goose_lang/typing.v
@@ -629,3 +629,7 @@ the first according to the GooseLang semantics. *)
 Reserved Notation "l +ₗ[ t ] z" (at level 50, left associativity, format "l  +ₗ[ t ]  z").
 Notation "l +ₗ[ t ] z" := (l +ₗ ty_size t * z) : stdpp_scope .
 Notation "e1 +ₗ[ t ] e2" := (BinOp (OffsetOp (ty_size t)) e1%E e2%E) : expr_scope .
+
+Lemma byte_offset_untype `{ext_ty: ext_types} l z :
+  l +ₗ[byteT] z = l +ₗ z.
+Proof. rewrite Z.mul_1_l. done. Qed.
